Prove that the sexp encoding produces valid sexps
Provable because of the additional string encoding. Also, showed one
piece of the fact that if the strings don't contain unprintable
characters or backslashes then the additional encoding is redundant.

compiler/parsing/fromSexpScript.sml
@@ -310,11 +310,38 @@ val encode_decode_control = Q.store_thm("encode_decode_control",
                (fn(a,t)=>`^(t"l") = ^(t"n")` by decide_tac)))
   \\ fs[]);
 
+val SEXSTR_def = Define`
+  SEXSTR s = SX_STR (encode_control s)`;
+
+val SEXSTR_11 = Q.store_thm("SEXSTR_11[simp]",
+  `SEXSTR s1 = SEXSTR s2 ⇔ s1 = s2`,
+  rw[SEXSTR_def]
+  \\ metis_tac[decode_encode_control,SOME_11]);
+
+val SEXSTR_distinct = Q.store_thm("SEXSTR_distinct[simp]",
+  `(SEXSTR s ≠ SX_SYM sym) ∧
+   (SEXSTR s ≠ SX_NUM num) ∧
+   (SEXSTR s ≠ SX_CONS a d) ∧
+   ((SEXSTR s = SX_STR s') ⇔ s' = encode_control s)`,
+  rw[SEXSTR_def,EQ_IMP_THM]);
+
+val odestSEXSTR_def = Define`
+  (odestSEXSTR (SX_STR s) = decode_control s) ∧
+  (odestSEXSTR _ = NONE)`;
+
+val encode_control_remove = Q.store_thm("encode_control_remove",
+  `∀s. EVERY isPrint s ∧ #"\\" ∉ set s ⇒ encode_control s = s`,
+  Induct \\ simp[encode_control_def]);
+
+val SEXSTR_remove = Q.store_thm("SEXSTR_remove",
+  `EVERY isPrint s ∧ #"\\" ∉ set s ⇒ SEXSTR s = SX_STR s`,
+  rw[SEXSTR_def,encode_control_remove]);
 
 val odestSXSTR_def = Define`
   (odestSXSTR (SX_STR s) = SOME s) ∧
   (odestSXSTR _ = NONE)
 `;
+
 val odestSXSYM_def = Define`
   (odestSXSYM (SX_SYM s) = SOME s) ∧
   (odestSXSYM _ = NONE)
@@ -413,7 +440,7 @@ val sexpid_def = Define`
        (guard (nm = "Short" ∧ LENGTH args = 1)
               (lift Short (p (EL 0 args))) ++
         guard (nm = "Long" ∧ LENGTH args = 2)
-              (lift2 Long (odestSXSTR (EL 0 args)) (p (EL 1 args))))
+              (lift2 Long (odestSEXSTR (EL 0 args)) (p (EL 1 args))))
     od
 `;
 
@@ -422,7 +449,7 @@ val sexptctor_def = Define`
     do
        (nm, args) <- dstrip_sexp s ;
        assert(nm = "TC_name" ∧ LENGTH args = 1);
-       lift TC_name (sexpid odestSXSTR (EL 0 args))
+       lift TC_name (sexpid odestSEXSTR (EL 0 args))
     od ++
     do
       nm <- odestSXSYM s ;
@@ -445,7 +472,7 @@ val sexptype_def = tDefine "sexptype" `
     do
        (s, args) <- dstrip_sexp s ;
        (guard (s = "Tvar" ∧ LENGTH args = 1)
-              (lift Tvar (odestSXSTR (EL 0 args))) ++
+              (lift Tvar (odestSEXSTR (EL 0 args))) ++
         guard (s = "Tvar_db" ∧ LENGTH args = 1)
               (lift Tvar_db (odestSXNUM (EL 0 args))) ++
         guard (s = "Tapp" ∧ LENGTH args = 2)
@@ -463,14 +490,14 @@ val sexptype_def = tDefine "sexptype" `
 val sexplit_def = Define`
   sexplit s =
     lift (IntLit o (&)) (odestSXNUM s) ++
-    lift StrLit (odestSXSTR s) ++
+    lift StrLit (odestSEXSTR s) ++
     do
       (nm,args) <- dstrip_sexp s;
       assert(LENGTH args = 1);
       guard (nm = "-") (OPTION_BIND (odestSXNUM (HD args)) (λn. if n = 0 then NONE else SOME (IntLit (-&n)))) ++
       guard (nm = "char")
             do
-              cs <- odestSXSTR (HD args);
+              cs <- odestSEXSTR (HD args);
               assert(LENGTH cs = 1);
               return (Char (HD cs))
             od ++
@@ -487,13 +514,13 @@ val sexplit_def = Define`
    Unclear if this sort of special-casing is ever likely to be helpful *)
 val sexppat_def = tDefine "sexppat" `
   sexppat s =
-    lift Pvar (odestSXSTR s) ++
+    lift Pvar (odestSEXSTR s) ++
     do
       (nm, args) <- dstrip_sexp s;
       guard (nm = "Plit" ∧ LENGTH args = 1)
             (lift Plit (sexplit (EL 0 args))) ++
       guard (nm = "Pcon" ∧ LENGTH args = 2)
-            (lift2 Pcon (sexpopt (sexpid odestSXSTR) (EL 0 args))
+            (lift2 Pcon (sexpopt (sexpid odestSEXSTR) (EL 0 args))
                         (sexplist sexppat (EL 1 args))) ++
       guard (nm = "Pref" ∧ LENGTH args = 1) (lift Pref (sexppat (EL 0 args)))
     od
@@ -565,12 +592,12 @@ val sexpexp_def = tDefine "sexpexp" `
             (lift Lit (sexplit (EL 0 args))) ++
       guard (nm = "Con" ∧ LENGTH args = 2)
             (lift2 Con
-                   (sexpopt (sexpid odestSXSTR) (EL 0 args))
+                   (sexpopt (sexpid odestSEXSTR) (EL 0 args))
                    (sexplist sexpexp (EL 1 args))) ++
       guard (nm = "Var" ∧ LENGTH args = 1)
-            (lift Var (sexpid odestSXSTR (EL 0 args))) ++
+            (lift Var (sexpid odestSEXSTR (EL 0 args))) ++
       guard (nm = "Fun" ∧ LENGTH args = 2)
-            (lift2 Fun (odestSXSTR (EL 0 args)) (sexpexp (EL 1 args))) ++
+            (lift2 Fun (odestSEXSTR (EL 0 args)) (sexpexp (EL 1 args))) ++
       guard (nm = "App" ∧ LENGTH args = 2)
             (lift2 App (sexpop (EL 0 args)) (sexplist sexpexp (EL 1 args))) ++
       guard (nm = "Log" ∧ LENGTH args = 3)
@@ -586,12 +613,12 @@ val sexpexp_def = tDefine "sexpexp" `
               (sexpexp (EL 0 args))
               (sexplist (sexppair sexppat sexpexp) (EL 1 args))) ++
       guard (nm = "Let" ∧ LENGTH args = 3)
-            (lift Let (sexpopt odestSXSTR (EL 0 args)) <*>
+            (lift Let (sexpopt odestSEXSTR (EL 0 args)) <*>
                       (sexpexp (EL 1 args)) <*>
                       (sexpexp (EL 2 args))) ++
       guard (nm = "Letrec" ∧ LENGTH args = 2)
             (lift2 Letrec
-              (sexplist (sexppair odestSXSTR (sexppair odestSXSTR sexpexp)) (EL 0 args))
+              (sexplist (sexppair odestSEXSTR (sexppair odestSEXSTR sexpexp)) (EL 0 args))
               (sexpexp (EL 1 args)))
     od
 `
@@ -617,9 +644,9 @@ val sexpexp_def = tDefine "sexpexp" `
 val sexptype_def_def = Define`
   sexptype_def =
   sexplist
-    (sexppair (sexplist odestSXSTR)
-      (sexppair odestSXSTR
-        (sexplist (sexppair odestSXSTR (sexplist sexptype)))))`;
+    (sexppair (sexplist odestSEXSTR)
+      (sexppair odestSEXSTR
+        (sexplist (sexppair odestSEXSTR (sexplist sexptype)))))`;
 
 val sexpdec_def = Define`
   sexpdec s =
@@ -628,15 +655,15 @@ val sexpdec_def = Define`
       guard (nm = "Dlet" ∧ LENGTH args = 2)
             (lift2 Dlet (sexppat (EL 0 args)) (sexpexp (EL 1 args))) ++
       guard (nm = "Dletrec" ∧ LENGTH args = 1)
-            (lift Dletrec (sexplist (sexppair odestSXSTR (sexppair odestSXSTR sexpexp)) (HD args))) ++
+            (lift Dletrec (sexplist (sexppair odestSEXSTR (sexppair odestSEXSTR sexpexp)) (HD args))) ++
       guard (nm = "Dtype" ∧ LENGTH args = 1)
             (lift Dtype (sexptype_def (HD args))) ++
       guard (nm = "Dtabbrev" ∧ LENGTH args = 3)
-            (lift Dtabbrev (sexplist odestSXSTR (EL 0 args)) <*>
-                           (odestSXSTR (EL 1 args)) <*>
+            (lift Dtabbrev (sexplist odestSEXSTR (EL 0 args)) <*>
+                           (odestSEXSTR (EL 1 args)) <*>
                            (sexptype (EL 2 args))) ++
       guard (nm = "Dexn" ∧ LENGTH args = 2)
-            (lift2 Dexn (odestSXSTR (EL 0 args)) (sexplist sexptype (EL 1 args)))
+            (lift2 Dexn (odestSEXSTR (EL 0 args)) (sexplist sexptype (EL 1 args)))
     od`;
 
 val sexpspec_def = Define`
@@ -645,24 +672,24 @@ val sexpspec_def = Define`
        (nm, args) <- dstrip_sexp s ;
        if nm = "Sval" then
          guard (LENGTH args = 2)
-               (lift2 Sval (odestSXSTR (HD args)) (sexptype (EL 1 args)))
+               (lift2 Sval (odestSEXSTR (HD args)) (sexptype (EL 1 args)))
        else if nm = "Stype" then
          guard (LENGTH args = 1)
                (lift Stype (sexptype_def (HD args)))
        else if nm = "Stabbrev" then
          guard (LENGTH args = 3)
                (lift Stabbrev
-                       (sexplist odestSXSTR (HD args)) <*>
-                       (odestSXSTR (EL 1 args)) <*>
+                       (sexplist odestSEXSTR (HD args)) <*>
+                       (odestSEXSTR (EL 1 args)) <*>
                        (sexptype (EL 2 args)))
        else if nm = "Stype_opq" then
          guard (LENGTH args = 2)
                (lift2 Stype_opq
-                      (sexplist odestSXSTR (EL 0 args))
-                      (odestSXSTR (EL 1 args)))
+                      (sexplist odestSEXSTR (EL 0 args))
+                      (odestSEXSTR (EL 1 args)))
        else if nm = "Sexn" then
          guard (LENGTH args = 2)
-               (lift2 Sexn (odestSXSTR (EL 0 args))
+               (lift2 Sexn (odestSEXSTR (EL 0 args))
                       (sexplist sexptype (EL 1 args)))
        else fail
     od
@@ -675,7 +702,7 @@ val sexptop_def = Define`
         if nm = "Tmod" then
           do
              assert (LENGTH args = 3);
-             modN <- odestSXSTR (HD args);
+             modN <- odestSEXSTR (HD args);
              specopt <- sexpopt (sexplist sexpspec) (EL 1 args);
              declist <- sexplist sexpdec (EL 2 args);
              return (Tmod modN specopt declist)
@@ -707,8 +734,8 @@ val optsexp_11 = Q.store_thm("optsexp_11[simp]",
   cases_on `o1` >> cases_on `o2` >> fs[optsexp_def, listsexp_def]);
 
 val idsexp_def = Define`
-  (idsexp (Short n) = listsexp [SX_SYM"Short"; SX_STR n]) ∧
-  (idsexp (Long ns n) = listsexp [SX_SYM"Long"; SX_STR ns; SX_STR n])`;
+  (idsexp (Short n) = listsexp [SX_SYM"Short"; SEXSTR n]) ∧
+  (idsexp (Long ns n) = listsexp [SX_SYM"Long"; SEXSTR ns; SEXSTR n])`;
 
 val idsexp_11 = Q.store_thm("idsexp_11[simp]",
   `∀ i1 i2. idsexp i1 = idsexp i2 ⇔ i1 = i2`,
@@ -733,7 +760,7 @@ val tctorsexp_11 = Q.store_thm("tctorsexp_11[simp]",
   Induct >> gen_tac >> cases_on `t2` >> fs[tctorsexp_def, listsexp_def]);
 
 val typesexp_def = tDefine"typesexp"`
-  (typesexp (Tvar s) = listsexp [SX_SYM "Tvar"; SX_STR s]) ∧
+  (typesexp (Tvar s) = listsexp [SX_SYM "Tvar"; SEXSTR s]) ∧
   (typesexp (Tvar_db n) = listsexp [SX_SYM "Tvar_db"; SX_NUM n]) ∧
   (typesexp (Tapp ts ct) = listsexp [SX_SYM "Tapp"; listsexp (MAP typesexp ts); tctorsexp ct])`
   (WF_REL_TAC`measure t_size` >>
@@ -756,8 +783,8 @@ val litsexp_def = Define`
   (litsexp (IntLit i) =
    if i < 0 then listsexp [SX_SYM "-"; SX_NUM (Num(-i))]
             else SX_NUM (Num i)) ∧
-  (litsexp (Char c) = listsexp [SX_SYM "char"; SX_STR [c]]) ∧
-  (litsexp (StrLit s) = SX_STR s) ∧
+  (litsexp (Char c) = listsexp [SX_SYM "char"; SEXSTR [c]]) ∧
+  (litsexp (StrLit s) = SEXSTR s) ∧
   (litsexp (Word8 w) = listsexp [SX_SYM "word8"; SX_NUM (w2n w)])`;
 
 val litsexp_11 = Q.store_thm("litsexp_11[simp]",
@@ -766,7 +793,7 @@ val litsexp_11 = Q.store_thm("litsexp_11[simp]",
   \\ intLib.COOPER_TAC);
 
 val patsexp_def = tDefine"patsexp"`
-  (patsexp (Pvar s) = SX_STR s) ∧
+  (patsexp (Pvar s) = SEXSTR s) ∧
   (patsexp (Plit l) = listsexp [SX_SYM "Plit"; litsexp l]) ∧
   (patsexp (Pcon cn ps) = listsexp [SX_SYM "Pcon"; optsexp (OPTION_MAP idsexp cn); listsexp (MAP patsexp ps)]) ∧
   (patsexp (Pref p) = listsexp [SX_SYM "Pref"; patsexp p])`
@@ -848,15 +875,15 @@ val expsexp_def = tDefine"expsexp"`
   (expsexp (Lit l) = listsexp [SX_SYM "Lit"; litsexp l]) ∧
   (expsexp (Con cn es) = listsexp [SX_SYM "Con"; optsexp (OPTION_MAP idsexp cn); listsexp (MAP expsexp es)]) ∧
   (expsexp (Var id) = listsexp [SX_SYM "Var"; idsexp id]) ∧
-  (expsexp (Fun x e) = listsexp [SX_SYM "Fun"; SX_STR x; expsexp e]) ∧
+  (expsexp (Fun x e) = listsexp [SX_SYM "Fun"; SEXSTR x; expsexp e]) ∧
   (expsexp (App op es) = listsexp [SX_SYM "App"; opsexp op; listsexp (MAP expsexp es)]) ∧
   (expsexp (Log lop e1 e2) = listsexp [SX_SYM "Log"; lopsexp lop; expsexp e1; expsexp e2]) ∧
   (expsexp (If e1 e2 e3) = listsexp [SX_SYM "If"; expsexp e1; expsexp e2; expsexp e3]) ∧
   (expsexp (Mat e pes) = listsexp [SX_SYM "Mat"; expsexp e; listsexp (MAP (λ(p,e). SX_CONS (patsexp p) (expsexp e)) pes)]) ∧
-  (expsexp (Let so e1 e2) = listsexp [SX_SYM "Let"; optsexp (OPTION_MAP SX_STR so); expsexp e1; expsexp e2]) ∧
+  (expsexp (Let so e1 e2) = listsexp [SX_SYM "Let"; optsexp (OPTION_MAP SEXSTR so); expsexp e1; expsexp e2]) ∧
   (expsexp (Letrec funs e) = listsexp
     [SX_SYM "Letrec";
-     listsexp (MAP (λ(x,y,z). SX_CONS (SX_STR x) (SX_CONS (SX_STR y) (expsexp z))) funs);
+     listsexp (MAP (λ(x,y,z). SX_CONS (SEXSTR x) (SX_CONS (SEXSTR y) (expsexp z))) funs);
      expsexp e])`
   (WF_REL_TAC`measure exp_size` >>
    rpt conj_tac >> simp[] >>
@@ -875,14 +902,14 @@ val expsexp_11 = Q.store_thm("expsexp_11[simp]",
   \\ imp_res_tac (REWRITE_RULE[AND_IMP_INTRO] MAP_EQ_MAP_IMP)
   \\ TRY(first_x_assum match_mp_tac \\ rw[FORALL_PROD])
   \\ rpt(pairarg_tac \\ fs[])
-  \\ metis_tac[OPTION_MAP_INJ,idsexp_11,simpleSexpTheory.sexp_11]);
+  \\ metis_tac[OPTION_MAP_INJ,idsexp_11,simpleSexpTheory.sexp_11,SEXSTR_11]);
 
 val type_defsexp_def = Define`
   type_defsexp = listsexp o
     MAP (λ(xs,x,ls).
-      SX_CONS (listsexp (MAP SX_STR xs))
-        (SX_CONS (SX_STR x)
-          (listsexp (MAP (λ(y,ts). SX_CONS (SX_STR y) (listsexp (MAP typesexp ts))) ls))))`;
+      SX_CONS (listsexp (MAP SEXSTR xs))
+        (SX_CONS (SEXSTR x)
+          (listsexp (MAP (λ(y,ts). SX_CONS (SEXSTR y) (listsexp (MAP typesexp ts))) ls))))`;
 
 val type_defsexp_11 = Q.store_thm("type_defsexp_11[simp]",
   `∀t1 t2. type_defsexp t1 = type_defsexp t2 ⇔ t1 = t2`,
@@ -893,7 +920,7 @@ val type_defsexp_11 = Q.store_thm("type_defsexp_11[simp]",
   \\ rpt (pairarg_tac \\ fs[]) \\ rveq
   \\ conj_tac
   >- (
-    Q.ISPEC_THEN`SX_STR`match_mp_tac INJ_MAP_EQ
+    Q.ISPEC_THEN`SEXSTR`match_mp_tac INJ_MAP_EQ
     \\ simp[INJ_DEF] )
   \\ imp_res_tac (REWRITE_RULE[AND_IMP_INTRO] MAP_EQ_MAP_IMP)
   \\ first_x_assum match_mp_tac
@@ -906,10 +933,10 @@ val decsexp_def = Define`
   (decsexp (Dlet p e) = listsexp [SX_SYM "Dlet"; patsexp p; expsexp e]) ∧
   (decsexp (Dletrec funs) =
      listsexp [SX_SYM "Dletrec";
-               listsexp (MAP (λ(f,x,e). SX_CONS (SX_STR f) (SX_CONS (SX_STR x) (expsexp e))) funs)]) ∧
+               listsexp (MAP (λ(f,x,e). SX_CONS (SEXSTR f) (SX_CONS (SEXSTR x) (expsexp e))) funs)]) ∧
   (decsexp (Dtype td) = listsexp [SX_SYM "Dtype"; type_defsexp td]) ∧
-  (decsexp (Dtabbrev ns x t) = listsexp [SX_SYM "Dtabbrev"; listsexp (MAP SX_STR ns); SX_STR x; typesexp t]) ∧
-  (decsexp (Dexn x ts) = listsexp [SX_SYM "Dexn"; SX_STR x; listsexp (MAP typesexp ts)])`;
+  (decsexp (Dtabbrev ns x t) = listsexp [SX_SYM "Dtabbrev"; listsexp (MAP SEXSTR ns); SEXSTR x; typesexp t]) ∧
+  (decsexp (Dexn x ts) = listsexp [SX_SYM "Dexn"; SEXSTR x; listsexp (MAP typesexp ts)])`;
 
 val decsexp_11 = Q.store_thm("decsexp_11[simp]",
   `∀d1 d2. decsexp d1 = decsexp d2 ⇔ d1 = d2`,
@@ -919,11 +946,11 @@ val decsexp_11 = Q.store_thm("decsexp_11[simp]",
   \\ rpt(pairarg_tac \\ fs[]));
 
 val specsexp_def = Define`
-  (specsexp (Sval x t) = listsexp [SX_SYM "Sval"; SX_STR x; typesexp t]) ∧
+  (specsexp (Sval x t) = listsexp [SX_SYM "Sval"; SEXSTR x; typesexp t]) ∧
   (specsexp (Stype t) = listsexp [SX_SYM "Stype"; type_defsexp t]) ∧
-  (specsexp (Stabbrev ns x t) = listsexp [SX_SYM "Stabbrev"; listsexp (MAP SX_STR ns); SX_STR x; typesexp t]) ∧
-  (specsexp (Stype_opq ns x) = listsexp [SX_SYM "Stype_opq"; listsexp (MAP SX_STR ns); SX_STR x]) ∧
-  (specsexp (Sexn x ts) = listsexp [SX_SYM "Sexn"; SX_STR x; listsexp (MAP typesexp ts)])`;
+  (specsexp (Stabbrev ns x t) = listsexp [SX_SYM "Stabbrev"; listsexp (MAP SEXSTR ns); SEXSTR x; typesexp t]) ∧
+  (specsexp (Stype_opq ns x) = listsexp [SX_SYM "Stype_opq"; listsexp (MAP SEXSTR ns); SEXSTR x]) ∧
+  (specsexp (Sexn x ts) = listsexp [SX_SYM "Sexn"; SEXSTR x; listsexp (MAP typesexp ts)])`;
 
 val specsexp_11 = Q.store_thm("specsexp_11[simp]",
   `∀s1 s2. specsexp s1 = specsexp s2 ⇔ s1 = s2`,
@@ -935,7 +962,7 @@ val specsexp_11 = Q.store_thm("specsexp_11[simp]",
 
 val topsexp_def = Define`
   (topsexp (Tmod modN specopt declist) =
-     listsexp [SX_SYM "Tmod"; SX_STR modN; optsexp (OPTION_MAP (listsexp o MAP specsexp) specopt);
+     listsexp [SX_SYM "Tmod"; SEXSTR modN; optsexp (OPTION_MAP (listsexp o MAP specsexp) specopt);
                listsexp (MAP decsexp declist)]) ∧
   (topsexp (Tdec dec) =
      listsexp [SX_SYM "Tdec"; decsexp dec])`;
@@ -956,9 +983,18 @@ val odestSXSTR_SOME = Q.store_thm("odestSXSTR_SOME[simp]",
   `odestSXSTR s = SOME y ⇔ (s = SX_STR y)`,
   Cases_on`s`>>simp[odestSXSTR_def])
 
+val odestSEXSTR_SOME = Q.store_thm("odestSEXSTR_SOME[simp]",
+  `odestSEXSTR s = SOME y ⇔ (s = SEXSTR y)`,
+  Cases_on`s`\\simp[odestSEXSTR_def,SEXSTR_def]
+  \\ metis_tac[decode_encode_control,encode_decode_control]);
+
 val odestSXSTR_SX_STR = Q.store_thm("odestSXSTR_SX_STR[simp]",
   `odestSXSTR (SX_STR s) = SOME s`,
   rw[odestSXSTR_def])
+
+val odestSEXSTR_SEXSTR = Q.store_thm("odestSEXSTR_SEXSTR[simp]",
+  `odestSEXSTR (SEXSTR s) = SOME s`,
+  rw[odestSEXSTR_def]);
 
 val odestSXNUM_SX_NUM = Q.store_thm("odestSXNUM_SX_NUM[simp]",
   `odestSXNUM (SX_NUM n) = SOME n`,
@@ -972,8 +1008,16 @@ val odestSXNUM_SX_STR = Q.store_thm("odestSXNUM_SX_STR[simp]",
   `odestSXNUM (SX_STR s) = NONE`,
   EVAL_TAC)
 
+val odestSXNUM_SEXSTR = Q.store_thm("odestSXNUM_SEXSTR[simp]",
+  `odestSXNUM (SEXSTR s) = NONE`,
+  EVAL_TAC)
+
 val odestSXSTR_listsexp = Q.store_thm("odestSXSTR_listsexp[simp]",
   `odestSXSTR (listsexp l) = NONE`,
+  Cases_on`l`>>EVAL_TAC)
+
+val odestSEXSTR_listsexp = Q.store_thm("odestSEXSTR_listsexp[simp]",
+  `odestSEXSTR (listsexp l) = NONE`,
   Cases_on`l`>>EVAL_TAC)
 
 val odestSXNUM_listsexp = Q.store_thm("odestSXNUM_listsexp[simp]",
@@ -982,6 +1026,10 @@ val odestSXNUM_listsexp = Q.store_thm("odestSXNUM_listsexp[simp]",
 
 val dstrip_sexp_SX_STR = Q.store_thm("dstrip_sexp_SX_STR[simp]",
   `dstrip_sexp (SX_STR s) = NONE`,
+  EVAL_TAC)
+
+val dstrip_sexp_SEXSTR = Q.store_thm("dstrip_sexp_SEXSTR[simp]",
+  `dstrip_sexp (SEXSTR s) = NONE`,
   EVAL_TAC)
 
 val strip_sxcons_listsexp = Q.store_thm("strip_sxcons_listsexp[simp]",
@@ -1019,9 +1067,9 @@ val sexpopt_optsexp = Q.store_thm("sexpopt_optsexp[simp]",
    (sexpopt f (optsexp (OPTION_MAP g x)) = SOME x)`,
   Cases_on`x`>>EVAL_TAC >> simp[])
 
-val sexpid_odestSXSTR_idsexp = Q.store_thm("sexpid_odestSXSTR_idsexp[simp]",
-  `sexpid odestSXSTR (idsexp i) = SOME i`,
-  Cases_on`i` >> EVAL_TAC)
+val sexpid_odestSEXSTR_idsexp = Q.store_thm("sexpid_odestSEXSTR_idsexp[simp]",
+  `sexpid odestSEXSTR (idsexp i) = SOME i`,
+  Cases_on`i` >> simp[sexpid_def,idsexp_def]);
 
 val sexptctor_tctorsexp = Q.store_thm("sexptctor_tctorsexp[simp]",
   `sexptctor (tctorsexp t) = SOME t`,
@@ -1183,7 +1231,7 @@ val litsexp_sexplit = Q.store_thm("litsexp_sexplit",
   >- (
     rw[litsexp_def]
     \\ Cases_on`s` \\ fs[odestSXNUM_def] )
-  \\ reverse(Cases_on`odestSXSTR s`) \\ fs[]
+  \\ reverse(Cases_on`odestSEXSTR s`) \\ fs[]
   >- ( rw[litsexp_def])
   \\ pairarg_tac \\ fs[OPTION_IGNORE_BIND_OPTION_GUARD]
   \\ every_case_tac \\ fs[] \\ rw[litsexp_def]
@@ -1195,8 +1243,8 @@ val litsexp_sexplit = Q.store_thm("litsexp_sexplit",
   \\ every_case_tac \\ fs[] \\ rw[]
   \\ Cases_on`e1` \\ fs[odestSXNUM_def]);
 
-val idsexp_sexpid_odestSXSTR = Q.store_thm("idsexp_sexpid_odestSXSTR",
-  `sexpid odestSXSTR x = SOME y ⇒ x = idsexp y`,
+val idsexp_sexpid_odestSEXSTR = Q.store_thm("idsexp_sexpid_odestSEXSTR",
+  `sexpid odestSEXSTR x = SOME y ⇒ x = idsexp y`,
   rw[sexpid_def]
   \\ fs[dstrip_sexp_SOME] \\ rw[]
   \\ fs[]
@@ -1217,7 +1265,7 @@ val patsexp_sexppat = Q.store_thm("patsexp_sexppat",
   \\ pop_assum mp_tac
   \\ rw[Once sexppat_def]
   \\ fs[OPTION_IGNORE_BIND_OPTION_GUARD]
-  \\ reverse(Cases_on`odestSXSTR s`) \\ fs[]
+  \\ reverse(Cases_on`odestSEXSTR s`) \\ fs[]
   >- ( rw[patsexp_def] )
   \\ pairarg_tac \\ fs[]
   \\ every_case_tac \\ fs[] \\ rw[]
@@ -1234,7 +1282,7 @@ val patsexp_sexppat = Q.store_thm("patsexp_sexppat",
   >- (
     Cases_on`x`\\fs[optsexp_def,sexpopt_def,odestSXSYM_def,listsexp_def,dstrip_sexp_SOME]
     \\ rveq \\ fs[OPTION_IGNORE_BIND_OPTION_GUARD]
-    \\ imp_res_tac idsexp_sexpid_odestSXSTR )
+    \\ imp_res_tac idsexp_sexpid_odestSEXSTR )
   \\ fs[Once strip_sxcons_def]
   \\ every_case_tac \\ fs[] \\ rw[]
   \\ imp_res_tac sexplist_SOME \\ rw[]
@@ -1286,7 +1334,7 @@ val expsexp_sexpexp = Q.store_thm("expsexp_sexpexp",
   \\ rveq \\ fs[listsexp_def] \\ fs[GSYM listsexp_def]
   \\ rpt(match1_tac strip_sxcons_mtac)
   \\ imp_res_tac litsexp_sexplit
-  \\ imp_res_tac idsexp_sexpid_odestSXSTR
+  \\ imp_res_tac idsexp_sexpid_odestSEXSTR
   \\ imp_res_tac opsexp_sexpop
   \\ imp_res_tac sexplist_SOME
   \\ imp_res_tac sexpopt_SOME
@@ -1306,13 +1354,13 @@ val expsexp_sexpexp = Q.store_thm("expsexp_sexpexp",
     \\ metis_tac[MEM_EL] )
   \\ every_case_tac \\ fs[] \\ rw[]
   \\ fs[IS_SOME_EXISTS]
-  \\ imp_res_tac idsexp_sexpid_odestSXSTR
+  \\ imp_res_tac idsexp_sexpid_odestSEXSTR
   \\ fs[OPTION_APPLY_MAP2,OPTION_APPLY_MAP3]
   \\ fs[] \\ rveq
   \\ rw[expsexp_def,listsexp_def]
   \\ imp_res_tac sexpopt_SOME
   \\ every_case_tac \\ fs[IS_SOME_EXISTS]
-  \\ rw[] \\ fs[odestSXSTR_def]
+  \\ rw[] \\ fs[odestSEXSTR_def]
   \\ imp_res_tac lopsexp_sexplop);
 
 val tctorsexp_sexptctor = Q.store_thm("tctorsexp_sexptctor",
@@ -1334,7 +1382,7 @@ val tctorsexp_sexptctor = Q.store_thm("tctorsexp_sexptctor",
   \\ rveq \\ fs[]
   \\ match1_tac strip_sxcons_mtac
   \\ simp[tctorsexp_def,listsexp_def]
-  \\ imp_res_tac idsexp_sexpid_odestSXSTR
+  \\ imp_res_tac idsexp_sexpid_odestSEXSTR
   \\ rw[]);
 
 val typesexp_sexptype = Q.store_thm("typesexp_sexptype",
@@ -1473,5 +1521,128 @@ val topsexp_sexptop = Q.store_thm("topsexp_sexptop",
   \\ rw[] \\ rfs[EL_MAP]
   \\ fs[EL_MAP]
   \\ metis_tac[specsexp_sexpspec]);
+
+(* valid sexps *)
+
+val SEXSTR_valid = Q.store_thm("SEXSTR_valid[simp]",
+  `valid_sexp (SEXSTR s)`,
+  rw[SEXSTR_def,EVERY_isPrint_encode_control]);
+
+val listsexp_valid = Q.store_thm("listsexp_valid",
+  `∀ls. EVERY valid_sexp ls ⇒ valid_sexp (listsexp ls)`,
+  Induct \\ simp[listsexp_def] \\ simp[GSYM listsexp_def]
+  \\ EVAL_TAC);
+
+val idsexp_valid = Q.store_thm("idsexp_valid[simp]",
+  `∀i. valid_sexp (idsexp i)`,
+  Cases \\ simp[idsexp_def]
+  \\ match_mp_tac listsexp_valid
+  \\ simp[]
+  \\ EVAL_TAC);
+
+val tctorsexp_valid = Q.store_thm("tctorsexp_valid[simp]",
+  `∀t. valid_sexp (tctorsexp t)`,
+  Cases \\ simp[tctorsexp_def]
+  \\ TRY(match_mp_tac listsexp_valid)
+  \\ simp[]
+  \\ EVAL_TAC);
+
+val typesexp_valid = Q.store_thm("typesexp_valid[simp]",
+  `∀t. valid_sexp (typesexp t)`,
+  ho_match_mp_tac(theorem"typesexp_ind")
+  \\ rw[typesexp_def]
+  \\ match_mp_tac listsexp_valid
+  \\ simp[]
+  \\ rpt conj_tac
+  \\ TRY (match_mp_tac listsexp_valid)
+  \\ simp[EVERY_MAP,EVERY_MEM]
+  \\ EVAL_TAC);
+
+val litsexp_valid = Q.store_thm("litsexp_valid[simp]",
+  `∀l. valid_sexp (litsexp l)`,
+  Cases \\ rw[litsexp_def]
+  \\ match_mp_tac listsexp_valid
+  \\ rw[] \\ EVAL_TAC);
+
+val optsexp_valid = Q.store_thm("optsexp_valid",
+  `∀x. (∀y. x = SOME y ⇒ valid_sexp y) ⇒ valid_sexp (optsexp x)`,
+  Cases \\ rw[optsexp_def]
+  \\ TRY(match_mp_tac listsexp_valid) \\ rw[]
+  \\ EVAL_TAC);
+
+val patsexp_valid = Q.store_thm("patsexp_valid[simp]",
+  `∀p. valid_sexp (patsexp p)`,
+  ho_match_mp_tac(theorem"patsexp_ind")
+  \\ rw[patsexp_def]
+  \\ match_mp_tac listsexp_valid
+  \\ rw[]
+  \\ TRY (match_mp_tac optsexp_valid \\ rw[] \\ rw[])
+  \\ TRY (match_mp_tac listsexp_valid \\ simp[EVERY_MAP,EVERY_MEM])
+  \\ EVAL_TAC);
+
+val type_defsexp_valid = Q.store_thm("type_defsexp_valid[simp]",
+  `∀t. valid_sexp (type_defsexp t)`,
+  rw[type_defsexp_def]
+  \\ match_mp_tac listsexp_valid
+  \\ rw[EVERY_MEM,EVERY_MAP]
+  \\ pairarg_tac \\ rw[]
+  \\ match_mp_tac listsexp_valid
+  \\ rw[EVERY_MEM,EVERY_MAP]
+  \\ pairarg_tac \\ rw[]
+  \\ match_mp_tac listsexp_valid
+  \\ rw[EVERY_MEM,EVERY_MAP]);
+
+val opsexp_valid = Q.store_thm("opsexp_valid[simp]",
+  `∀op. valid_sexp (opsexp op)`,
+  Cases \\ simp[opsexp_def]
+  \\ TRY (EVAL_TAC \\ NO_TAC)
+  \\ Cases_on`o'` \\ simp[opsexp_def]
+  \\ EVAL_TAC);
+
+val lopsexp_valid = Q.store_thm("lopsexp_valid[simp]",
+  `∀l. valid_sexp (lopsexp l)`,
+  Cases \\ simp[lopsexp_def]
+  \\ EVAL_TAC);
+
+val expsexp_valid = Q.store_thm("expsexp_valid[simp]",
+  `∀e. valid_sexp (expsexp e)`,
+  ho_match_mp_tac(theorem"expsexp_ind")
+  \\ rw[expsexp_def]
+  \\ TRY(match_mp_tac listsexp_valid)
+  \\ rw[]
+  \\ TRY(EVAL_TAC \\ NO_TAC)
+  \\ TRY(match_mp_tac optsexp_valid \\ rw[] \\ rw[])
+  \\ TRY(match_mp_tac listsexp_valid \\ simp[EVERY_MAP,EVERY_MEM])
+  \\ simp[FORALL_PROD]
+  \\ first_x_assum MATCH_ACCEPT_TAC);
+
+val decsexp_valid = Q.store_thm("decsexp_valid[simp]",
+  `∀d. valid_sexp (decsexp d)`,
+  Cases \\ simp[decsexp_def]
+  \\ match_mp_tac listsexp_valid
+  \\ rw[]
+  \\ TRY (EVAL_TAC \\ NO_TAC)
+  \\ match_mp_tac listsexp_valid
+  \\ simp[EVERY_MAP,EVERY_MEM]
+  \\ simp[FORALL_PROD]);
+
+val specsexp_valid = Q.store_thm("specsexp_valid[simp]",
+  `∀s. valid_sexp (specsexp s)`,
+  Cases \\ simp[specsexp_def]
+  \\ match_mp_tac listsexp_valid
+  \\ rw[]
+  \\ TRY(EVAL_TAC \\ NO_TAC)
+  \\ match_mp_tac listsexp_valid
+  \\ simp[EVERY_MAP]);
+
+val topsexp_valid = Q.store_thm("topsexp_valid[simp]",
+  `∀t. valid_sexp (topsexp t)`,
+  Cases \\ simp[topsexp_def]
+  \\ match_mp_tac listsexp_valid
+  \\ rw[]
+  \\ TRY(EVAL_TAC \\ NO_TAC)
+  \\ TRY(match_mp_tac optsexp_valid \\ rw[])
+  \\ match_mp_tac listsexp_valid
+  \\ simp[EVERY_MAP,EVERY_MEM]);
 
 val _ = export_theory();
